Implemented [FDSerial] as an intermediate spec

proofs/TriangularToSerialFD.v
@@ -30,13 +30,20 @@ Section SerialFD.
   Variables addrSize dataBytes rfIdx: nat.
   Variable decodeInst: DecodeT dataBytes rfIdx.
 
-  Section Fetch.
-    Variables (iMemReqName f2dName: string).
+  Definition f2trName := "f2tr".
+  Definition tr2dName := "tr2d".
 
-    Definition F2D :=
-      STRUCT { "f2dOrig" :: Struct (F2D addrSize);
-               "iMemReq" :: Struct (RqFromProc addrSize dataBytes) }.
-    Definition f2dEnq := MethodSig (f2dName -- "enq")(Struct F2D): Void.
+  Definition F2Tr :=
+    STRUCT { "f2dOrig" :: Struct (F2D addrSize);
+             "iMemReq" :: Struct (RqFromProc addrSize dataBytes) }.
+
+  Definition Tr2D :=
+    STRUCT { "f2dOrig" :: Struct (F2D addrSize);
+             "iMemRep" :: Struct (RsToProc dataBytes) }.
+
+  Section Fetch.
+
+    Definition f2trEnq := MethodSig (f2trName -- "enq")(Struct F2Tr): Void.
 
     Definition btbPredPc := btbPredPc addrSize.
     Definition redirGet := redirGet addrSize.
@@ -54,7 +61,7 @@ Section SerialFD.
           Call decEpoch <- (getEpoch "dec")();
           Call exeEpoch <- (getEpoch "exe")();
           Call resetException();
-          Call f2dEnq (
+          Call f2trEnq (
                  STRUCT { "f2dOrig" ::= STRUCT { "pc" ::= #pc;
                                                  "predPc" ::= #predPc;
                                                  "decEpoch" ::= #decEpoch;
@@ -93,6 +100,147 @@ Section SerialFD.
 
   End Fetch.
 
+  Section FDTrans.
+    Definition f2trDeq := MethodSig (f2trName -- "deq")(): Struct F2Tr.
+    Definition tr2dEnq := MethodSig (tr2dName -- "enq")(Struct Tr2D): Void.
+    Definition exec :=
+      MethodSig "exec"(Struct (RqFromProc addrSize dataBytes)) : Struct (RsToProc dataBytes).
+
+    Definition fdtrans :=
+      MODULE {
+        Rule "processLd" :=
+          Call f2tr <- f2trDeq();
+          LET f2dOrig <- #f2tr!F2Tr@."f2dOrig";
+          LET req <- #f2tr!F2Tr@."iMemReq";
+          Assert !#req!(RqFromProc addrSize dataBytes)@."op";
+          Call rep <- exec(#req);
+          Call tr2dEnq(STRUCT { "f2dOrig" ::= #f2dOrig;
+                                "iMemRep" ::= #rep });
+          Retv
+            
+        with Rule "processSt" :=
+          Call f2tr <- f2trDeq();
+          LET f2dOrig <- #f2tr!F2Tr@."f2dOrig";
+          LET req <- #f2tr!F2Tr@."iMemReq";
+          Assert #req!(RqFromProc addrSize dataBytes)@."op";
+          Call rep <- exec(#req);
+          Call tr2dEnq(STRUCT { "f2dOrig" ::= #f2dOrig;
+                                "iMemRep" ::= #rep });
+          Retv
+      }.
+
+  End FDTrans.
+
+  Section Decode.
+    Definition tr2dDeq := MethodSig (tr2dName -- "deq")(): Struct Tr2D.
+
+    Definition DecodedInst := decodedInst dataBytes rfIdx.
+
+    Definition D2R := D2R addrSize dataBytes rfIdx.
+    Definition d2rEnq := d2rEnq addrSize dataBytes rfIdx d2rName.
+    Definition bhtPredTaken := bhtPredTaken addrSize.
+
+    Definition decodeSerial :=
+      MODULE {
+        Rule "doDecode" :=
+          Call tr2d <- tr2dDeq();
+          LET f2d <- #tr2d!Tr2D@."f2dOrig";
+          LET pc <- #f2d!(F2D addrSize)@."pc";
+          LET instStr <- #tr2d!Tr2D@."iMemRep";
+          LET inst <- #instStr!(RsToProc dataBytes)@."data";
+
+          Call decEpoch <- (getEpoch "dec")();
+          Call exeEpoch <- (getEpoch "exe")();
+
+          If (#exeEpoch == #f2d!(F2D addrSize)@."exeEpoch"
+              && #decEpoch == #f2d!(F2D addrSize)@."decEpoch")
+          then
+            LET predPc <- #f2d!(F2D addrSize)@."predPc";
+            LET dInst <- decodeInst _ inst;
+
+            If (#dInst!DecodedInst@."iType" != $$iTypeUnsupported)
+            then
+              If (#dInst!DecodedInst@."iType" == $$iTypeBr)
+              then
+                Call taken <- bhtPredTaken(#pc);
+                LET bhtPredPc : Bit addrSize <-
+                  (IF #taken
+                   then #pc + UniBit (ZeroExtendTrunc _ _)
+                                     #dInst!DecodedInst@."imm"
+                   else #pc + $4);
+                If (#predPc != #bhtPredPc)
+                then
+                  LET ret : Struct (Maybe (Bit addrSize)) <- STRUCT { "isValid" ::= $$true;
+                                                                      "value" ::= #bhtPredPc };
+                  Ret #ret
+                else (* #predPc == #bhtPredPc *)
+                  LET ret : Struct (Maybe (Bit addrSize)) <- STRUCT { "isValid" ::= $$false;
+                                                                      "value" ::= $$Default };
+                  Ret #ret
+                as ret;
+                Ret #ret
+              else (* #dInst!DecodedInst@."iType" != $$iTypeBr *)
+                If (#dInst!DecodedInst@."iType" == $$iTypeJ)
+                then
+                  LET jumpAddr <- #pc + UniBit (ZeroExtendTrunc _ _)
+                                               #dInst!DecodedInst@."imm";
+                  If (#predPc != #jumpAddr)
+                  then
+                    LET ret : Struct (Maybe (Bit addrSize)) <- STRUCT { "isValid" ::= $$true;
+                                                                        "value" ::= #jumpAddr };
+                    Ret #ret
+                  else (* #predPc == #jumpAddr *)
+                    LET ret : Struct (Maybe (Bit addrSize)) <- STRUCT { "isValid" ::= $$false;
+                                                                        "value" ::= $$Default };
+                    Ret #ret
+                  as ret;
+                  Ret #ret
+                else (* #dInst!DecodedInst@."iType" != $$iTypeJ *)
+                  Ret (STRUCT { "isValid" ::= $$false; "value" ::= $$Default })
+                as ret;
+                Ret #ret
+              as ret;
+
+              If (#ret!(Maybe (Bit addrSize))@."isValid")
+              then
+                Call (redirSetValid addrSize "dec")(
+                       STRUCT { "pc" ::= #pc;
+                                "nextPc" ::= #ret!(Maybe (Bit addrSize))@."value" });
+                Call d2rEnq(STRUCT { "pc" ::= #pc;
+                                     "predPc" ::= #ret!(Maybe (Bit addrSize))@."value";
+                                     "dInst" ::= #dInst;
+                                     "exeEpoch" ::= #exeEpoch });
+                Retv
+              else (* ! #ret!(Maybe (Bit addrSize))@."isValid" *)
+                Call d2rEnq(STRUCT { "pc" ::= #pc;
+                                     "predPc" ::= #predPc;
+                                     "dInst" ::= #dInst;
+                                     "exeEpoch" ::= #exeEpoch });
+                Retv;
+              Retv
+            else (* #dInst!DecodedInst@."iType" == $$iTypeUnsupported *)
+              Call setException($$excIllegalInst);
+              Retv;
+            Retv;
+          Retv
+      }.
+
+  End Decode.
+
+  (** The serial implementation *)
+  Definition FDSerial :=
+    (fetchSerial ++ fdtrans ++ decodeSerial)%kami.
+
 End SerialFD.
 
+Section Correctness.
+  Variables addrSize dataBytes rfIdx: nat.
+  Variable decodeInst: DecodeT dataBytes rfIdx.
+
+  Lemma fd_implements_fdSerial:
+    (FD addrSize decodeInst) <<== (FDSerial addrSize decodeInst).
+  Proof.
+  Admitted.
+
+End Correctness.
 
